Adequacy and Standard Termination-Insensitive NI
- Added an indexed multi relation and its relation to the standard multi relation.
- Added an Adequacy theorem for the indexed multi step.
- Lifted Preservation to the bridge relation.
- Added auxiliary TINI Lemma for the indexed relation via adequacy.
- Standard TINI is a shown by relating standard multi relation
  to the indexed one and then using the auxiliary TINI Lemma.

Bridge.v
@@ -1,46 +1,10 @@
-Require Import Bool Arith List CpdtTactics SfLib LibTactics.
+Require Import Bool Arith List CpdtTactics SfLib LibTactics Omega.
 Require Import Coq.Program.Equality.
 
 Set Implicit Arguments.
 
 Require Import Identifier Environment Imperative Types Augmented.
 
-(* 
-Inductive obs :=
-  | Halt : obs
-  | Effect : {  evt | evt <> EmptyEvent } -> obs.
-
-
-Print Effect.
-
-
-Lemma eq_obs_dec: forall ev1 ev2: obs, {ev1 = ev2} + { ev1<>ev2 }.
-Proof.
-  decide equality.
-
-Qed.
-Local Hint Resolve eq_obs_dec.
-
-
-Definition is_effect (o:obs) :Prop :=
-  exists ℓ x v, o = Effect ℓ x v.
-
-Definition is_low_effect (o: obs) : Prop :=
-  exists x v, o = Effect Low x v.
-
-
-Lemma low_effects_are_effects:
-  forall o,
-    is_low_effect o -> is_effect o.
-Proof.
-  intros.
-  unfold is_effect.
-  unfold is_low_effect in *.
-  exists Low.
-  auto.
-Qed.
-Hint Resolve low_effects_are_effects : Sec.
- *)
 
 Inductive low_event : typenv -> level -> event -> Prop :=
 | low_assigment_is_low_event:
@@ -53,25 +17,10 @@ Definition high_event Γ ℓ evt := ~low_event Γ ℓ evt.
 Definition low_event_step  Γ ℓ evt cfg cfg' := event_step Γ evt cfg cfg' /\ low_event Γ ℓ evt.
 Definition high_event_step Γ ℓ evt cfg cfg' := event_step Γ evt cfg cfg' /\ high_event Γ ℓ evt.
 
-(*
-Inductive bridge_step:
-  typenv -> level -> config -> config -> event -> Prop:=
-| bridge_low :
-    forall Γ ℓ evt cfg cfg',
-      low_event_step Γ ℓ evt cfg cfg' ->
-      bridge_step Γ ℓ cfg cfg' evt
-| bridge_stop :
-    forall Γ ℓ evt cfg cfg',
-      high_event_step Γ ℓ evt cfg cfg' ->
-      is_stop_config cfg' ->
-      bridge_step Γ ℓ cfg cfg' evt
-| bridge_trans:
-    forall Γ ℓ evt' evt'' cfg cfg' cfg'',
-      high_event_step Γ ℓ evt' cfg cfg' ->
-      is_not_stop_config cfg' ->
-      bridge_step Γ ℓ evt'' cfg' cfg'' ->
-      bridge_step Γ ℓ evt'' cfg cfg''.
-*)
+Hint Constructors low_event.
+Hint Unfold high_event.
+Hint Unfold high_event_step.
+Hint Unfold low_event_step.
 
 
 Inductive bridge_step_num:
@@ -112,9 +61,6 @@ Notation " t '⇒+/(SL,' Γ ',' obs ')'  t' " :=
   (bridge_step Γ Low t t' obs) (at level 40).
 
 
-(* Not sure if we will need this after all *)
-
-
 (* Multi-step reduction *)
 
 Inductive multi {X:Type} (R: relation X): relation X :=
@@ -123,7 +69,7 @@ Inductive multi {X:Type} (R: relation X): relation X :=
          R x y ->
          multi R y z ->
          multi R x z.
-Local Hint Resolve multi_refl.
+Hint Resolve multi_refl.
 
 
 Tactic Notation "multi_cases" tactic(first) ident(c) :=
@@ -159,3 +105,75 @@ Qed.
 (* Multi-step transitions *)
 Definition multistep := multi step.
 Notation " t '⇒*' t' " := (multistep t t') (at level 40).
+
+
+
+
+
+
+Definition relation_idx := fun X : Type => X -> X -> nat -> Prop.
+
+Inductive multi_idx {X:Type} (R: relation X) :relation_idx X :=
+   | multi_refl_zero : forall (x : X), multi_idx R x x 0
+   | multi_step_more : forall (x y z : X) n,
+                         R x y ->
+                         multi_idx R y z n ->
+                         multi_idx R x z (S n).
+
+
+Hint Resolve multi_refl_zero.
+
+
+Tactic Notation "multi_idx_cases" tactic(first) ident(c) :=
+  first;
+  [ Case_aux c "multi_refl_zero" | Case_aux c "multi_step_more" ].
+
+
+
+(* Multi-step transitions *)
+Definition multistep_idx := multi_idx step.
+Notation " t '⇒/+' n '+/' s" := (multi_idx step t s n) (at level 40).
+
+
+Theorem multi_idx_R:
+  forall (X:Type) (R: relation X) ( x y : X),
+    R x y -> (multi_idx R) x y 1.
+Proof.                     
+  intros.
+  eapply multi_step_more; eauto.
+Qed.  
+
+Theorem multi_idx_trans:
+  forall n (X: Type) (R: relation X) ( x y z: X ) m,
+    multi_idx R x y n ->
+    multi_idx R y z m ->
+    multi_idx R x z (n + m).
+Proof.    
+  intros n X R.
+  induction n; intros.
+  -     inverts* H.
+        
+  - inversion H; subst; auto.
+    assert (multi_idx R x y0 1) by (econstructor; eauto).
+    
+    specialize (IHn y0 y z m H5 H0).
+    replace (S n + m) with (S (n + m)) by omega.
+    eapply multi_step_more; eauto.
+Qed.    
+
+
+Theorem from_multi_to_multi_idx:
+  forall (X:Type) (R:relation X) (x y : X),
+    multi R x y -> exists n, (multi_idx R x y n).
+Proof.
+  intros.
+  induction H.
+  - (exists 0; constructor).
+  - destruct IHmulti as [n ?IHmulti].
+    (exists (S n)).
+    econstructor; eauto.
+Qed.
+
+(* TODO: 2016-07-28: move multi_idx someplace else *)
+
+
