Adequacy.v
@@ -1,0 +1,207 @@
+(** Adequacy of the bridge semantics w.r.t. standard semantics for
+well-typed programs.
+
+Author: Aslan Askarov 
+Created: 2016-07-27
+
+- Note: that well-typedness is required may potentially be relaxed, 
+  but we leave that for future investigation.
+
+ *) 
+
+
+
+Require Import Bool Arith List CpdtTactics SfLib LibTactics.
+Require Import Coq.Program.Equality.
+Require Import Omega.
+
+Set Implicit Arguments.
+
+Require Import Identifier Environment Imperative Types Augmented Bridge.
+Require Import WellFormedness LowEq NIexp.
+Require Import InductionPrinciple.
+Require Import UtilTactics.
+Require Import BridgeTactics.
+Require Import BridgeProperties.
+Require Import HighPCSteps.
+
+
+Lemma adequacy_of_event_steps:
+  forall Γ pc c m cfg',
+    wf_mem m Γ ->
+    -{ Γ, pc ⊢ c }- ->
+    〈c, m 〉 ⇒ cfg' ->
+    exists ev, event_step Γ ev 〈c, m 〉 cfg'.
+Proof.
+  intros Γ pc c m [c' m']; intros.
+  cmd_cases (dependent induction c) Case.
+  Case "STOP".
+  { invert_step. }
+  Case "SKIP".
+  { exists EmptyEvent.
+    assert (c' = STOP /\ m' = m).
+    {
+      inverts H1.
+      splits~.
+    }
+    super_destruct. subst.
+    constructor; auto.
+  }
+  Case "::=".
+  {
+    inverts keep H1.
+    inverts H0.
+    exists (AssignmentEvent ℓ' i v).
+    constructor~.
+  }
+  Case ";;".
+  { assert (-{ Γ, pc ⊢ c1 }-) by
+        (match goal with [ H:  -{ Γ, pc ⊢ c1;; c2 }- |- _ ] => inverts keep H end; auto).
+    inverts H1;
+      repeat match goal
+           with
+             | [ H:  〈 c1, m 〉 ⇒ 〈 ?c1', m' 〉|- _  ] =>
+                  (specializes IHc1 m c1' m' H;
+                   destruct IHc1 as [ev];
+                   (exists ev);
+                   constructor~ )
+             |  [ H:  -{ Γ, pc ⊢ c1;; c' }- |- _ ] =>
+                ( inverts H;
+                  applys* wt_programs_are_not_stop
+                )
+           end.
+  }
+  Case "IFB".
+  {
+    exists EmptyEvent.
+    assert (c' = c1 \/ c' = c2) as H_cmd
+        by (inverts keep H1; tauto).
+    match goal with
+      | [ H:  -{ Γ, pc ⊢ IFB e THEN c1 ELSE c2 FI }- |- _ ]
+        => inverts keep H
+    end.
+    assert (  -{ Γ, pc ⊢ c' }- )
+      by ( destruct H_cmd; subst; applys* pc_lowering).
+
+    assert ( m = m') by (inverts* H1); subst.
+    constructor~ .
+    applys* wt_programs_are_not_stop.
+  }
+  Case "WHILE".
+  {
+    exists EmptyEvent.
+    inverts keep H1.
+    constructor~ .
+    crush.
+  }
+Qed.   
+
+(* TODO: 2016-07-28: simplify the above lemma *)
+
+
+
+(* Multi-N relation *)
+
+
+Theorem bridge_adequacy:
+  forall Γ (n:nat) c m m_end ,
+    〈c, m 〉 ⇒/+ n +/ 〈STOP, m_end 〉 ->
+    forall pc, -{ Γ, pc ⊢ c }-  ->
+    wf_mem m Γ  ->
+    (c = STOP \/
+     exists ev n' cfg' k,
+       〈 c, m 〉 ⇨+/(SL, Γ, ev, n') cfg' /\
+       cfg' ⇒/+ k +/ 〈STOP, m_end 〉 /\ k < n).
+
+Proof.
+  intros Γ n.
+
+
+  dependent induction n.
+  (* n = 0 *)
+  { 
+    left~. 
+    inverts H. auto.
+  }
+
+
+  (* inductive case *)
+  {
+    right; subst.
+    inversion H.
+    
+    
+    match goal with  [ H : 〈 c, m 〉 ⇒ ?y |- _ ] => destruct y as [c' m'] end; subst.
+    match goal with [ H:  〈 c', m' 〉 ⇒/+ n +/ 〈 STOP, m_end 〉 |- _ ] => rename H into H_n end.
+    match goal with [ H:  〈 c, m 〉 ⇒ 〈c', m' 〉 |- _ ] => rename H into H_step end.
+
+    
+    specialize (IHn c' m' m_end H_n pc).
+        
+    lets* (ev & H_ev) : adequacy_of_event_steps H_step.
+
+    (* We define two auxiliary local propositions that consider the
+       cases of a high and a low event respectively; these are then
+       used in the case analysis afterwards *)
+
+    assert ( low_event Γ Low ev ->
+              exists ev0 n' cfg' k,
+                〈 c, m 〉 ⇨+/(SL, Γ, ev0, n') cfg' /\ cfg' ⇒/+ k +/ 〈 STOP, m_end 〉/\ k < S n) as LemmaLowEvent.
+    {
+      intros H_low.
+      inverts H_low.
+      assert (ℓ' = Low) by
+        ( destruct ℓ'; auto; try impossible_flows; subst ); subst.
+      (exists   (AssignmentEvent Low x u) 1).
+      forwards* (H_wf' & H_wt' ): preservation.
+      compare c' STOP; intros;subst.
+      * clear IHn.
+
+        
+        lets : multi_idx_stop_trivial H_n; subst.
+        (exists*〈STOP, m_end 〉0).
+        splits~ ; try omega.
+        applys~ bridge_low_num.
+
+      * specializes~ H_wt' __ .
+        specializes~ H_n.
+        exists 〈c', m' 〉.
+        exists n.
+        splits~ .
+        applys* bridge_low_num.
+    }
+
+    assert ( high_event Γ Low ev ->
+              exists ev0 n' cfg' k,
+                〈 c, m 〉 ⇨+/(SL, Γ, ev0, n') cfg' /\ cfg' ⇒/+ k +/ 〈 STOP, m_end 〉/\ k < S n) as LemmaHighEvent.
+    { clear LemmaLowEvent.
+      intros H_high.
+      compare c' STOP; intros; subst.
+      - (exists EmptyEvent 1 〈STOP, m' 〉 0).
+        lets : multi_idx_stop_trivial H_n; subst.
+        splits~ ; try omega.
+        applys*  bridge_stop_num.
+      - forwards*   (H_wf' & H_wt') : preservation. 
+        specializes~ H_wt'.
+        specializes~ IHn.
+        destruct* IHn as [? | ?IHH_multi].
+
+        lets (?ev' & ?n' &  ?cfg' & k & ?H_bridge & ?H_tail & ?H_k ): IHH_multi.
+        exists ev' (S n') cfg' k.
+        splits~ ; try omega.
+        applys* bridge_trans_num.
+    }
+    
+    
+    (* now we are ready to do the case analysis of the event, using the above assertions *)
+    destruct ev.
+    - (* Empty Event *)
+      apply* LemmaHighEvent.
+    - (* Assignment Event *)
+      destruct l.
+      + (* l is Low *)
+        apply* LemmaLowEvent.
+      + (* l is High *)
+        applys* LemmaHighEvent.
+  }
+Qed.
