BridgeTactics.v
@@ -1,7 +1,7 @@
-(* 
+(*
 
-General tactics to help discharge properties about Bridge relation 
-Author: Aslan Askarov 
+General tactics to help discharge properties about Bridge relation
+Author: Aslan Askarov
 Created: 2016-07-26
 
 *)
@@ -35,7 +35,7 @@ Ltac invert_high_steps :=
     end.
 
 
-   
+
 
 
 Ltac stop_contradiction:=
@@ -90,10 +90,182 @@ Ltac _find keyword:=
   match goal with
     | [H : context [keyword] |- _ ] => H
   end.
-  
+
 
 Ltac _eapply_in_ctxt keyw what :=
   let H := _find (keyw)
   in eapply what in H.
 
 
+
+
+(* LEMMAS that go into Hints *)
+
+Lemma is_stop_trivial : forall m, is_stop_config 〈STOP, m 〉.
+            Proof.
+              intros.
+              match goal with
+                | [ |- is_stop_config 〈STOP, ?m 〉 ] =>
+                unfolds; exists m; tauto
+              end.
+              Qed.
+
+Hint Resolve is_stop_trivial.
+
+
+
+
+Lemma is_not_stop_config_inversion:
+  forall c st,
+    is_not_stop_config 〈c, st 〉 ->
+    c <> STOP.
+  intros.
+  match goal with
+      [H : is_not_stop_config 〈 ?c, ?st 〉 |-  ?c <> STOP ] =>
+      (do 2 unfolds in H);
+        unfolds is_stop_config;
+        unfold not;
+        intros;
+        destruct H;
+        exists st;
+        congruence
+  end.
+Qed.
+
+Hint Resolve is_not_stop_config_inversion.
+
+
+Lemma is_stop_config_inversion:
+  forall c st,
+    is_stop_config 〈c, st 〉 ->
+    c = STOP.
+  intros.
+  unfolds in H.
+  destruct H.
+  congruence.
+Qed.
+
+Hint Resolve is_stop_config_inversion.
+
+
+Lemma empty_event_is_high :
+  forall Γ,
+  high_event Γ Low EmptyEvent.
+Proof.
+  intros.
+  do 2 unfolds; intros;
+  match goal with [H : context [low_event] |- _ ] => inverts H end.
+Qed.
+
+Hint Resolve empty_event_is_high.
+
+
+
+
+Lemma bridge_steps_are_positive:
+         forall Γ c m ev n cfg,
+           〈 c, m 〉 ⇨+/(SL, Γ, ev, n) cfg ->
+           n >= 1.
+         Proof.
+           intros.
+           inverts* H.
+Qed.
+Hint Resolve bridge_steps_are_positive.
+
+
+Lemma is_non_stop_config_trivial:
+         forall c st,
+           c <> STOP ->
+           is_not_stop_config 〈c, st 〉.
+Proof.
+         intros.
+         do 2 unfolds.
+         intros.
+         inversion H0.
+         inversion H1.
+         subst.
+         tauto.
+       Qed.
+Hint Resolve is_non_stop_config_trivial.
+
+
+Lemma multi_stop_trivial:
+  forall m m',
+    〈 STOP, m 〉⇒*〈STOP, m' 〉 ->
+    m = m'.
+Proof.
+  intros.
+  inverts* H.
+  inverts H0.
+Qed.
+Hint Resolve multi_stop_trivial.
+
+
+Lemma multi_idx_stop_trivial:
+   forall m m' n,
+    〈 STOP, m 〉⇒/+ n +/ 〈STOP, m' 〉 ->
+    m = m'.
+Proof.
+  intros.
+  inverts* H.
+  inversion H0.
+Qed.
+Hint Resolve multi_idx_stop_trivial.
+
+Lemma high_assignments_are_high_events:
+  forall Γ x u,
+    high_event Γ Low (AssignmentEvent High x u).
+Proof.
+  intros.
+  do 2 unfolds.
+  intros.
+  inversion H.
+  subst.
+  impossible_flows.
+Qed.
+Hint Resolve high_assignments_are_high_events.
+
+
+
+
+(*)
+
+Lemma is_not_stop_config_inversion:
+  forall c st,
+    is_not_stop_config 〈c, st 〉 ->
+    c <> STOP.
+  intros.
+  match goal with
+      [H : is_not_stop_config 〈 ?c, ?st 〉 |-  ?c <> STOP ] =>
+      (do 2 unfolds in H);
+        unfolds is_stop_config;
+        unfold not;
+        intros;
+        destruct H;
+        exists st;
+        congruence
+  end.
+Qed.
+
+
+
+Lemma is_stop_config_inversion:
+  forall c st,
+    is_stop_config 〈c, st 〉 ->
+    c = STOP.
+  intros.
+  unfolds in H.
+  destruct H.
+  congruence.
+Qed.
+
+
+Lemma empty_event_is_high :
+  forall Γ,
+  high_event Γ Low EmptyEvent.
+Proof.
+  intros.
+  do 2 unfolds; intros;
+  match goal with [H : context [low_event] |- _ ] => inverts H end.
+Qed.
+*)
