NI.v
@@ -1,0 +1,125 @@
+(* Top-level noninterference 
+   Author: Aslan Askarov
+   Created: 2016-07-28
+ *)
+Require Import Bool Arith List CpdtTactics SfLib LibTactics.
+Require Import Coq.Program.Equality.
+Require Import Omega.
+
+Set Implicit Arguments.
+
+Require Import Identifier Environment Imperative Types Augmented Bridge.
+Require Import WellFormedness LowEq NIexp.
+Require Import InductionPrinciple.
+Require Import UtilTactics.
+Require Import BridgeTactics.
+Require Import BridgeProperties.
+Require Import HighPCSteps.
+Require Import Adequacy.
+Require Import NIBridge.
+
+
+Definition TINI_idx (n: nat): Prop :=  
+  forall Γ c m m_end s s_end pc k,
+    〈c, m 〉 ⇒/+ n +/ 〈STOP, m_end 〉 ->
+    -{ Γ, pc ⊢ c }- ->
+    state_low_eq Γ m s ->
+    〈c, s 〉 ⇒/+ k +/ 〈STOP, s_end 〉 ->
+    state_low_eq Γ m_end s_end.
+
+Lemma tini_idx: forall n, TINI_idx (n).
+
+Proof.
+  apply strongind.
+  (* base case *)
+  { unfolds.
+    intros.
+    inverts H.
+    inverts H0.
+  }
+  (* inductive case *)
+  {
+    
+    unfold TINI_idx.
+    intros n IH Γ c m m_end s s_end pc k H_m H_wt H_leq H_s. 
+
+    forwards* H_bridge_m: bridge_adequacy H_m.
+    {
+      inverts~ H_leq.
+    }
+
+    forwards* H_bridge_s: bridge_adequacy H_s.
+    {
+      inverts~ H_leq.
+    }
+
+    (* TODO: 2016-07-29 : complete the case by applying ni_bridge_num *) 
+    
+    destruct H_bridge_m as [? | ?H_bridge_m];
+      subst ;
+      try  (solve [inverts H_wt]).
+    destruct H_bridge_s as [? | ?H_bridge_s];
+      subst;
+      try  (solve [inverts H_wt]).
+    
+
+    
+    lets  (?ev1 & ?n1 &  ?cfg1 & ?k1 & ?H_bridge_IH1 & H_multi_IH1 & ?): H_bridge_m.
+    lets  (?ev2 & ?n2 &  ?cfg2 & ?k2 & ?H_bridge_IH2 & H_multi_IH2 & ?): H_bridge_s.
+
+    (* TODO apply the same to H_bridge_m *)
+    (* TODO: earlier : add stop non-typability into hints *)
+    
+    clear H_bridge_m H_bridge_s.
+
+    destruct cfg1 as [c1 m'].
+    destruct cfg2 as [c2 s'].
+      
+      
+    assert (k1 <= n) as H_k1 by omega.
+
+    replace n1 with (S (n1 - 1)) in * by (inverts* H_bridge_IH1; omega ).
+    replace n2 with (S (n2 - 1)) in * by (inverts* H_bridge_IH2; omega ).
+
+    lets NI_bridge: ni_bridge_num (n1 -1); unfold NI_idx in NI_bridge.
+
+
+        
+    specializes~ NI_bridge (>>Γ c m s ev1  c1  m' s' (n2 - 1) ___).
+
+
+    forwards* (? & ?H_wt'): preservation_bridge.
+    {
+      inversion H_leq; auto.
+    }
+    lets (H_leq' & cmd_eq & ? ) : NI_bridge.
+    clear NI_bridge.
+    subst.
+    
+    compare c2 STOP; intros; subst.
+    - assert (m' = m_end) by eauto.
+      assert (s' = s_end) by eauto.
+      subst*.
+    - specializes* H_wt'.
+  }
+Qed.
+
+    
+(* Standard termination-insensitive noninterference *)
+
+Theorem TINI:
+  forall Γ c m s m_end s_end pc,
+    -{ Γ, pc ⊢ c }- ->
+    state_low_eq Γ m s ->
+    〈c, m 〉 ⇒* 〈STOP, m_end 〉 ->
+    〈c, s 〉 ⇒* 〈STOP, s_end 〉 ->
+    state_low_eq Γ m_end s_end.
+Proof.    
+  intros Γ c m s m_end s_end pc H_wt H_leq H_m H_s.
+  forwards (?n & ?H'_m) : from_multi_to_multi_idx H_m; clear H_m.
+  forwards (?k & ?H'_s) : from_multi_to_multi_idx H_s; clear H_s.
+
+  applys tini_idx H'_m H_wt H_leq H'_s.
+Qed.
+
+     
